Risc0/Gadgets/ComputeDecode/Witness/WeakestPreFull.lean
@@ -1,37 +1,40 @@
 import Risc0.Basic
 import Risc0.Gadgets.ComputeDecode.Witness.Code
+import Risc0.Gadgets.ComputeDecode.Witness.CodeReordered
+import Risc0.Gadgets.ComputeDecode.Witness.CodeParts
+import Risc0.Gadgets.ComputeDecode.Witness.CodeDrops
 import Risc0.Gadgets.ComputeDecode.Witness.WeakestPresPart0
 import Risc0.Gadgets.ComputeDecode.Witness.WeakestPresPart1
 import Risc0.Gadgets.ComputeDecode.Witness.WeakestPresPart2
 import Risc0.Gadgets.ComputeDecode.Witness.WeakestPresPart3
-import Risc0.Gadgets.ComputeDecode.Witness.WeakestPresPart4
-import Risc0.Gadgets.ComputeDecode.Witness.WeakestPresPart5
-import Risc0.Gadgets.ComputeDecode.Witness.WeakestPresPart6
-import Risc0.Gadgets.ComputeDecode.Witness.WeakestPresPart7
-import Risc0.Gadgets.ComputeDecode.Witness.WeakestPresPart8
-import Risc0.Gadgets.ComputeDecode.Witness.WeakestPresPart9
-import Risc0.Gadgets.ComputeDecode.Witness.WeakestPresPart10
-import Risc0.Gadgets.ComputeDecode.Witness.WeakestPresPart11
-import Risc0.Gadgets.ComputeDecode.Witness.WeakestPresPart12
-import Risc0.Gadgets.ComputeDecode.Witness.WeakestPresPart13
-import Risc0.Gadgets.ComputeDecode.Witness.WeakestPresPart14
-import Risc0.Gadgets.ComputeDecode.Witness.WeakestPresPart15
-import Risc0.Gadgets.ComputeDecode.Witness.WeakestPresPart16
-import Risc0.Gadgets.ComputeDecode.Witness.WeakestPresPart17
-import Risc0.Gadgets.ComputeDecode.Witness.WeakestPresPart18
-import Risc0.Gadgets.ComputeDecode.Witness.WeakestPresPart19
-import Risc0.Gadgets.ComputeDecode.Witness.WeakestPresPart20
-import Risc0.Gadgets.ComputeDecode.Witness.WeakestPresPart21
-import Risc0.Gadgets.ComputeDecode.Witness.WeakestPresPart22
-import Risc0.Gadgets.ComputeDecode.Witness.WeakestPresPart23
-import Risc0.Gadgets.ComputeDecode.Witness.WeakestPresPart24
-import Risc0.Gadgets.ComputeDecode.Witness.WeakestPresPart25
-import Risc0.Gadgets.ComputeDecode.Witness.WeakestPresPart26
-import Risc0.Gadgets.ComputeDecode.Witness.WeakestPresPart27
-import Risc0.Gadgets.ComputeDecode.Witness.WeakestPresPart28
-import Risc0.Gadgets.ComputeDecode.Witness.WeakestPresPart29
-import Risc0.Gadgets.ComputeDecode.Witness.WeakestPresPart30
-import Risc0.Gadgets.ComputeDecode.Witness.WeakestPresPart31
+-- import Risc0.Gadgets.ComputeDecode.Witness.WeakestPresPart4
+-- import Risc0.Gadgets.ComputeDecode.Witness.WeakestPresPart5
+-- import Risc0.Gadgets.ComputeDecode.Witness.WeakestPresPart6
+-- import Risc0.Gadgets.ComputeDecode.Witness.WeakestPresPart7
+-- import Risc0.Gadgets.ComputeDecode.Witness.WeakestPresPart8
+-- import Risc0.Gadgets.ComputeDecode.Witness.WeakestPresPart9
+-- import Risc0.Gadgets.ComputeDecode.Witness.WeakestPresPart10
+-- import Risc0.Gadgets.ComputeDecode.Witness.WeakestPresPart11
+-- import Risc0.Gadgets.ComputeDecode.Witness.WeakestPresPart12
+-- import Risc0.Gadgets.ComputeDecode.Witness.WeakestPresPart13
+-- import Risc0.Gadgets.ComputeDecode.Witness.WeakestPresPart14
+-- import Risc0.Gadgets.ComputeDecode.Witness.WeakestPresPart15
+-- import Risc0.Gadgets.ComputeDecode.Witness.WeakestPresPart16
+-- import Risc0.Gadgets.ComputeDecode.Witness.WeakestPresPart17
+-- import Risc0.Gadgets.ComputeDecode.Witness.WeakestPresPart18
+-- import Risc0.Gadgets.ComputeDecode.Witness.WeakestPresPart19
+-- import Risc0.Gadgets.ComputeDecode.Witness.WeakestPresPart20
+-- import Risc0.Gadgets.ComputeDecode.Witness.WeakestPresPart21
+-- import Risc0.Gadgets.ComputeDecode.Witness.WeakestPresPart22
+-- import Risc0.Gadgets.ComputeDecode.Witness.WeakestPresPart23
+-- import Risc0.Gadgets.ComputeDecode.Witness.WeakestPresPart24
+-- import Risc0.Gadgets.ComputeDecode.Witness.WeakestPresPart25
+-- import Risc0.Gadgets.ComputeDecode.Witness.WeakestPresPart26
+-- import Risc0.Gadgets.ComputeDecode.Witness.WeakestPresPart27
+-- import Risc0.Gadgets.ComputeDecode.Witness.WeakestPresPart28
+-- import Risc0.Gadgets.ComputeDecode.Witness.WeakestPresPart29
+-- import Risc0.Gadgets.ComputeDecode.Witness.WeakestPresPart30
+-- import Risc0.Gadgets.ComputeDecode.Witness.WeakestPresPart31
 
 namespace Risc0.ComputeDecode.Witness.WP
 
@@ -46,82 +49,137 @@ def start_state (input : BufferAtTime) : State :=
   , isFailed := false
   }
 
-open Lean Elab Tactic in
-elab "MLIR_witness_updates" : tactic => do
-  evalTactic <| ← `(
-    tactic| (
-      MLIR_states_new
-      simp [←Map.getElem_def, Map.update_get_next, Map.update_get_next', Map.update_get]
-      MLIR_decide_updates
-    )
-  )
-
 lemma closed_form {x₀ x₁ x₂ x₃: Felt} {y₀ y₁ y₂ y₃ y₄ y₅ y₆ y₇ y₈ y₉ y₁₀ y₁₁ y₁₂ y₁₃ y₁₄ y₁₅ y₁₆ y₁₇ : Option Felt} :
   Code.run (start_state [x₀, x₁, x₂, x₃]) = [y₀, y₁, y₂, y₃, y₄, y₅, y₆, y₇, y₈, y₉, y₁₀, y₁₁, y₁₂, y₁₃, y₁₄, y₁₅, y₁₆, y₁₇ ] ↔ sorry := by
+  unfold Code.run
+  rewrite [Code.optimised_behaviour1]
+  rewrite [Code.optimised_behaviour2]
+  rewrite [Code.optimised_behaviour3]
+  rewrite [Code.optimised_behaviour4]
+  rewrite [Code.optimised_behaviour5]
+  rewrite [Code.optimised_behaviour6]
+  rewrite [Code.optimised_behaviour7]
+  rewrite [Code.optimised_behaviour8]
+  rewrite [Code.optimised_behaviour9]
+  rewrite [Code.optimised_behaviour10]
+  rewrite [Code.optimised_behaviour11]
+  rewrite [Code.optimised_behaviour12]
+  rewrite [Code.optimised_behaviour13]
+  rewrite [Code.optimised_behaviour14]
+  rewrite [Code.optimised_behaviour15]
+  rewrite [Code.optimised_behaviour16]
+  rewrite [Code.optimised_behaviour17]
+  rewrite [Code.optimised_behaviour18]
+  rewrite [Code.optimised_behaviour19]
+  rewrite [Code.optimised_behaviour20]
+  rewrite [Code.optimised_behaviour21]
+  rewrite [Code.optimised_behaviour22]
+  rewrite [Code.optimised_behaviour23]
+  rewrite [Code.optimised_behaviour24]
+  rewrite [Code.optimised_behaviour25]
+  rewrite [Code.optimised_behaviour26]
+  rewrite [Code.optimised_behaviour27]
+  rewrite [Code.optimised_behaviour28]
+  rewrite [Code.optimised_behaviour29]
+  rewrite [Code.optimised_behaviour30]
+  rewrite [Code.optimised_behaviour31]
+  rewrite [Code.optimised_behaviour32]
+  unfold MLIR.runProgram
+  rewrite [←Code.parts_combine]
+  unfold Code.parts_combined
+  rewrite [←Code.getReturn_ignores_drops]
+  rewrite [←Code.behaviour_with_drops]
   rewrite [part0_wp]
   rewrite [part1_updates_opaque]
-  unfold start_state
-  unfold part0_state
+  unfold start_state part0_state
   MLIR_states_updates
 
   rewrite [part2_updates_opaque]
   unfold part1_state
   MLIR_states_updates
+  unfold part1_drops
+  simp [State.dropFelts]
+  MLIR_states_updates
+  simp only [Map.drop_base, ne_eq, Map.update_drop_swap, Map.update_drop]
+  rewrite [Map.drop_of_updates]
+  simp only [Map.drop_base, ne_eq, Map.update_drop_swap, Map.update_drop]
 
   rewrite [part3_updates_opaque]
   unfold part2_state
   MLIR_states_updates
-
-  rewrite [part4_updates_opaque]
-  unfold part3_state
+  unfold part2_drops
+  simp [State.dropFelts]
   MLIR_states_updates
+  simp only [ne_eq, Map.update_drop_swap, Map.update_drop, Map.drop_base]
+  rewrite [Map.drop_of_updates]
+  simp only [Map.drop_base, ne_eq, Map.update_drop_swap, Map.update_drop]
+  
 
-  rewrite [part5_updates_opaque]
-  unfold part4_state
-  MLIR_states_updates
+  -- Code.run (start_state [x₀, x₁, x₂, x₃]) = [y₀, y₁, y₂, y₃, y₄, y₅, y₆, y₇, y₈, y₉, y₁₀, y₁₁, y₁₂, y₁₃, y₁₄, y₁₅, y₁₆, y₁₇ ] ↔ sorry := by
+  -- rewrite [part0_wp]
+  -- rewrite [part1_updates_opaque]
+  -- unfold start_state
+  -- unfold part0_state
+  -- MLIR_states_updates
 
-  rewrite [part6_updates_opaque]
-  unfold part5_state
-  MLIR_states_updates
+  -- rewrite [part2_updates_opaque]
+  -- unfold part1_state
+  -- MLIR_states_updates
 
-  rewrite [part7_updates_opaque]
-  unfold part6_state
-  MLIR_states_updates
+  -- rewrite [part3_updates_opaque]
+  -- unfold part2_state
+  -- MLIR_states_updates
+
+  -- rewrite [part4_updates_opaque]
+  -- unfold part3_state
+  -- MLIR_states_updates
+
+  -- rewrite [part5_updates_opaque]
+  -- unfold part4_state
+  -- MLIR_states_updates
+
+  -- rewrite [part6_updates_opaque]
+  -- unfold part5_state
+  -- MLIR_states_updates
+
+  -- rewrite [part7_updates_opaque]
+  -- unfold part6_state
+  -- MLIR_states_updates
 
 
-  generalize h_none : [none, none, none, none, none, none, none, none, none, none, none, none, none, none, none, none, none, none] = nones
+  -- generalize h_none : [none, none, none, none, none, none, none, none, none, none, none, none, none, none, none, none, none, none] = nones
 
-  -- rewrite [part8_updates_opaque]
-  -- unfold part7_state
-  -- MLIR_witness_updates
+  -- -- rewrite [part8_updates_opaque]
+  -- -- unfold part7_state
+  -- -- MLIR_witness_updates
 
-  -- rewrite [part9_updates_opaque]
-  -- unfold part8_state
-  -- MLIR_witness_updates
+  -- -- rewrite [part9_updates_opaque]
+  -- -- unfold part8_state
+  -- -- MLIR_witness_updates
 
-  -- rewrite [part₃_updates_opaque]
-  -- rewrite [part₄_updates_opaque]
-  -- rewrite [part₅_updates_opaque]
+  -- -- rewrite [part₃_updates_opaque]
+  -- -- rewrite [part₄_updates_opaque]
+  -- -- rewrite [part₅_updates_opaque]
 
 
 
-  -- unfold part₁_state
-  -- MLIR_witness_updates
+  -- -- unfold part₁_state
+  -- -- MLIR_witness_updates
 
-  -- unfold part₂_state
-  -- MLIR_witness_updates
+  -- -- unfold part₂_state
+  -- -- MLIR_witness_updates
 
-  -- unfold part₃_state
-  -- MLIR_witness_updates
+  -- -- unfold part₃_state
+  -- -- MLIR_witness_updates
 
-  -- unfold part₄_state
-  -- MLIR_witness_updates
+  -- -- unfold part₄_state
+  -- -- MLIR_witness_updates
 
-  -- unfold part₅_state
-  -- MLIR_witness_updates
+  -- -- unfold part₅_state
+  -- -- MLIR_witness_updates
 
-  -- simp [State.lastOutput, Option.get!, List.getLast!, List.getLast, State.buffers]
-  -- MLIR_witness_updates
-  -- simp [List.getLast]
+  -- -- simp [State.lastOutput, Option.get!, List.getLast!, List.getLast, State.buffers]
+  -- -- MLIR_witness_updates
+  -- -- simp [List.getLast]
 
 end Risc0.ComputeDecode.Witness.WP
